\begin{frame}{Lösung 3}
	\framesubtitle{Ableitung aus Prämisse}
	Prämisse: $\Gamma =\{P\rightarrow(Q\rightarrow R), Q\}$, zz: $P\rightarrow R$\\
	\begin{tabular}{cl}
		\textcolor{blue}{$I_{Ax_{AL2}}$}           & $(P\rightarrow(Q\rightarrow R))\rightarrow((P\rightarrow Q)\rightarrow(P\rightarrow R))$ \\
		\textcolor{blue}{$IV_{\textit{Prämisse}}$} & $P\rightarrow(Q\rightarrow R)$                                                           \\
		\textcolor{blue}{$III_{MP(I, II)}$}        & $(P\rightarrow Q)\rightarrow(P\rightarrow R)$                                            \\
		\textcolor{blue}{$IV_{\textit{Prämisse}}$} & $Q$                                                                                      \\
		\textcolor{blue}{$V_{IV, Ax_{AL1}}$}       & $Q\rightarrow(P\rightarrow Q)$                                                           \\
		\textcolor{blue}{$VI_{MP(IV, V)}$}         & $P\rightarrow Q$                                                                         \\
		\textcolor{blue}{$VII_{MP(III, VI)}$}      & $P\rightarrow R$                                                                         \\
	\end{tabular}
	$Ax_{AL1} = (G\rightarrow(H\rightarrow G))$\\
	$Ax_{AL2} = (G\rightarrow(H\rightarrow K))\rightarrow((G\rightarrow H)\rightarrow(G\rightarrow K))$\\
\end{frame}
%I
\begin{frame}
	\frametitle{Lösung 3}
	\framesubtitle{Ableitung aus Prämisse}
	Prämisse: $\Gamma =\{P\rightarrow(Q\rightarrow R), Q\}$, zz: $P\rightarrow R$\\
	\begin{tabular}{cl}
		\textcolor{green}{$I_{Ax_{AL2}}$}           & $($\textcolor{red}{$P\rightarrow(Q\rightarrow R)$}$)\rightarrow((P\rightarrow Q)\rightarrow(P\rightarrow R))$ \\
		\textcolor{white}{$II_{\textit{Prämisse}}$} & \textcolor{white}{$P\rightarrow(Q\rightarrow R)$}                                                             \\
		\textcolor{white}{$III_{MP(I, II)}$}        & \textcolor{white}{$(P\rightarrow Q)\rightarrow(P\rightarrow R)$}                                              \\
		\textcolor{white}{$IV_{\textit{Prämisse}}$} & \textcolor{white}{$Q$}                                                                                        \\
		\textcolor{white}{$V_{IV, Ax_{AL1}}$}       & \textcolor{white}{$Q\rightarrow(P\rightarrow Q)$}                                                             \\
		\textcolor{white}{$VI_{MP(IV, V)}$}         & \textcolor{white}{$P\rightarrow Q$}                                                                           \\
		\textcolor{white}{$VII_{MP(III, VI)}$}      & \textcolor{white}{$P\rightarrow R$}                                                                           \\
	\end{tabular}
	$Ax_{AL1} = (G\rightarrow(H\rightarrow G))$\\
	$Ax_{AL2} = ($\textcolor{red}{$G\rightarrow(H\rightarrow K)$}$)\rightarrow((G\rightarrow H)\rightarrow(G\rightarrow K))$\\
\end{frame}
%II
\begin{frame}
	\frametitle{Lösung 3}
	\framesubtitle{Ableitung aus Prämisse}
	Prämisse: $\Gamma =\{$\textcolor{red}{$P\rightarrow(Q\rightarrow R)$}$, Q\}$, zz: $P\rightarrow R$\\
	\begin{tabular}{cl}
		\textcolor{blue}{$I_{Ax_{AL2}}$}            & $(P\rightarrow(Q\rightarrow R))\rightarrow((P\rightarrow Q)\rightarrow(P\rightarrow R))$ \\
		\textcolor{green}{$II_{\textit{Prämisse}}$} & \textcolor{red}{$P\rightarrow(Q\rightarrow R)$}                                          \\
		\textcolor{white}{$III_{MP(I, II)}$}        & \textcolor{white}{$(P\rightarrow Q)\rightarrow(P\rightarrow R)$}                         \\
		\textcolor{white}{$IV_{\textit{Prämisse}}$} & \textcolor{white}{$Q$}                                                                   \\
		\textcolor{white}{$V_{IV, Ax_{AL1}}$}       & \textcolor{white}{$Q\rightarrow(P\rightarrow Q)$}                                        \\
		\textcolor{white}{$VI_{MP(IV, V)}$}         & \textcolor{white}{$P\rightarrow Q$}                                                      \\
		\textcolor{white}{$VII_{MP(III, VI)}$}      & \textcolor{white}{$P\rightarrow R$}                                                      \\
	\end{tabular}
	$Ax_{AL1} = (G\rightarrow(H\rightarrow G))$\\
	$Ax_{AL2} = (G\rightarrow(H\rightarrow K))\rightarrow((G\rightarrow H)\rightarrow(G\rightarrow K))$\\
\end{frame}
%III
\begin{frame}
	\frametitle{Lösung 3}
	\framesubtitle{Ableitung aus Prämisse}
	Prämisse: $\Gamma =\{P\rightarrow(Q\rightarrow R), Q\}$, zz: $P\rightarrow R$\\
	\begin{tabular}{cl}
		\textcolor{blue}{$I_{Ax_{AL2}}$}            & $($\textcolor{gray}{$P\rightarrow(Q\rightarrow R)$}$)\rightarrow($\textcolor{red}{$(P\rightarrow Q)\rightarrow(P\rightarrow R)$}$)$ \\
		\textcolor{blue}{$II_{\textit{Prämisse}}$}  & \textcolor{gray}{$P\rightarrow(Q\rightarrow R)$}                                                                                    \\
		\textcolor{green}{$III_{MP(I, II)}$}        & \textcolor{red}{$(P\rightarrow Q)\rightarrow(P\rightarrow R)$}                                                                      \\
		\textcolor{white}{$IV_{\textit{Prämisse}}$} & \textcolor{white}{$Q$}                                                                                                              \\
		\textcolor{white}{$V_{IV, Ax_{AL1}}$}       & \textcolor{white}{$Q\rightarrow(P\rightarrow Q)$}                                                                                   \\
		\textcolor{white}{$VI_{MP(IV, V)}$}         & \textcolor{white}{$P\rightarrow Q$}                                                                                                 \\
		\textcolor{white}{$VII_{MP(III, VI)}$}      & \textcolor{white}{$P\rightarrow R$}                                                                                                 \\
	\end{tabular}
	$Ax_{AL1} = (G\rightarrow(H\rightarrow G))$\\
	$Ax_{AL2} = (G\rightarrow(H\rightarrow K))\rightarrow((G\rightarrow H)\rightarrow(G\rightarrow K))$\\
\end{frame}
%IV
\begin{frame}
	\frametitle{Lösung 3}
	\framesubtitle{Ableitung aus Prämisse}
	Prämisse: $\Gamma =\{P\rightarrow(Q\rightarrow R), $\textcolor{red}{$Q$}$\}$, zz: $P\rightarrow R$\\
	\begin{tabular}{cl}
		\textcolor{blue}{$I_{Ax_{AL2}}$}            & $(P\rightarrow(Q\rightarrow R))\rightarrow((P\rightarrow Q)\rightarrow(P\rightarrow R))$ \\
		\textcolor{blue}{$II_{\textit{Prämisse}}$}  & $P\rightarrow(Q\rightarrow R)$                                                           \\
		\textcolor{blue}{$III_{MP(I, II)}$}         & $(P\rightarrow Q)\rightarrow(P\rightarrow R)$                                            \\
		\textcolor{green}{$IV_{\textit{Prämisse}}$} & \textcolor{red}{$Q$}                                                                     \\
		\textcolor{white}{$V_{IV, Ax_{AL1}}$}       & \textcolor{white}{$Q\rightarrow(P\rightarrow Q)$}                                        \\
		\textcolor{white}{$VI_{MP(IV, V)}$}         & \textcolor{white}{$P\rightarrow Q$}                                                      \\
		\textcolor{white}{$VII_{MP(III, VI)}$}      & \textcolor{white}{$P\rightarrow R$}                                                      \\
	\end{tabular}
	$Ax_{AL1} = (G\rightarrow(H\rightarrow G))$\\
	$Ax_{AL2} = (G\rightarrow(H\rightarrow K))\rightarrow((G\rightarrow H)\rightarrow(G\rightarrow K))$\\
\end{frame}
%V
\begin{frame}
	\frametitle{Lösung 3}
	\framesubtitle{Ableitung aus Prämisse}
	Prämisse: $\Gamma =\{P\rightarrow(Q\rightarrow R), $\textcolor{red}{$Q$}$\}$, zz: $P\rightarrow R$\\
	\begin{tabular}{cl}
		\textcolor{blue}{$I_{Ax_{AL2}}$}           & $(P\rightarrow(Q\rightarrow R))\rightarrow((P\rightarrow Q)\rightarrow(P\rightarrow R))$ \\
		\textcolor{blue}{$II_{\textit{Prämisse}}$} & $P\rightarrow(Q\rightarrow R)$                                                           \\
		\textcolor{blue}{$III_{MP(I, II)}$}        & $(P\rightarrow Q)\rightarrow(P\rightarrow R)$                                            \\
		\textcolor{blue}{$IV_{\textit{Prämisse}}$} & $Q$                                                                                      \\
		\textcolor{green}{$V_{IV, Ax_{AL1}}$}      & \textcolor{red}{$Q$}$\rightarrow(P\rightarrow $\textcolor{red}{$Q$}$)$                   \\
		\textcolor{white}{$VI_{MP(IV, V)}$}        & \textcolor{white}{$P\rightarrow Q$}                                                      \\
		\textcolor{white}{$VII_{MP(III, VI)}$}     & \textcolor{white}{$P\rightarrow R$}                                                      \\
	\end{tabular}
	$Ax_{AL1} = ($\textcolor{red}{$G$}$\rightarrow(H\rightarrow $\textcolor{red}{$G$}$))$\\
	$Ax_{AL2} = (G\rightarrow(H\rightarrow K))\rightarrow((G\rightarrow H)\rightarrow(G\rightarrow K))$\\
\end{frame}
%VI
\begin{frame}
	\frametitle{Lösung 3}
	\framesubtitle{Ableitung aus Prämisse}
	Prämisse: $\Gamma =\{P\rightarrow(Q\rightarrow R), Q\}$, zz: $P\rightarrow R$\\
	\begin{tabular}{cl}
		\textcolor{blue}{$I_{Ax_{AL2}}$}           & $(P\rightarrow(Q\rightarrow R))\rightarrow((P\rightarrow Q)\rightarrow(P\rightarrow R))$ \\
		\textcolor{blue}{$II_{\textit{Prämisse}}$} & $P\rightarrow(Q\rightarrow R)$                                                           \\
		\textcolor{blue}{$III_{MP(I, II)}$}        & $(P\rightarrow Q)\rightarrow(P\rightarrow R)$                                            \\
		\textcolor{blue}{$IV_{\textit{Prämisse}}$} & \textcolor{gray}{$Q$}                                                                    \\
		\textcolor{blue}{$V_{IV, Ax_{AL1}}$}       & \textcolor{gray}{$Q$}$\rightarrow($\textcolor{red}{$P\rightarrow Q$}$)$                  \\
		\textcolor{green}{$VI_{MP(IV, V)}$}        & \textcolor{red}{$P\rightarrow Q$}                                                        \\
		\textcolor{white}{$VII_{MP(III, VI)}$}     & \textcolor{white}{$P\rightarrow R$}                                                      \\
	\end{tabular}
	$Ax_{AL1} = (G\rightarrow(H\rightarrow G))$\\
	$Ax_{AL2} = (G\rightarrow(H\rightarrow K))\rightarrow((G\rightarrow H)\rightarrow(G\rightarrow K))$\\
\end{frame}
%VII
\begin{frame}
	\frametitle{Lösung 3}
	\framesubtitle{Ableitung aus Prämisse}
	Prämisse: $\Gamma =\{P\rightarrow(Q\rightarrow R), Q\}$, zz: $P\rightarrow R$\\
	\begin{tabular}{cl}
		\textcolor{blue}{$I_{Ax_{AL2}}$}           & $(P\rightarrow(Q\rightarrow R))\rightarrow((P\rightarrow Q)\rightarrow(P\rightarrow R))$ \\
		\textcolor{blue}{$II_{\textit{Prämisse}}$} & $P\rightarrow(Q\rightarrow R)$                                                           \\
		\textcolor{blue}{$III_{MP(I, II)}$}        & $($\textcolor{gray}{$P\rightarrow Q$}$)\rightarrow($\textcolor{red}{$P\rightarrow R$}$)$ \\
		\textcolor{blue}{$IV_{\textit{Prämisse}}$} & $Q$                                                                                      \\
		\textcolor{blue}{$V_{IV, Ax_{AL1}}$}       & $Q\rightarrow(P\rightarrow Q)$                                                           \\
		\textcolor{blue}{$VI_{MP(IV, V)}$}         & \textcolor{gray}{$P\rightarrow Q$}                                                       \\
		\textcolor{green}{$VII_{MP(III, VI)}$}     & \textcolor{red}{$P\rightarrow R$}                                                        \\
	\end{tabular}
	$Ax_{AL1} = (G\rightarrow(H\rightarrow G))$\\
	$Ax_{AL2} = (G\rightarrow(H\rightarrow K))\rightarrow((G\rightarrow H)\rightarrow(G\rightarrow K))$\\
\end{frame}
