\begin{frame}{LÃ¶sung 1}
	$F = \neg((A\wedge B)\rightarrow\neg(B\vee A))$\\
	Definiere:\\
	\begin{itemize}
		\item $C:=A\wedge B$
		\item $D:=B\vee A$
		\item $E:=\neg D=\neg(B\vee A)$
		\item $G:=C\rightarrow E=(A\wedge B)\rightarrow\neg(B\vee A)$
	\end{itemize}
	$\Rightarrow F=\neg G$\\
	\begin{tabular}{cc|cccc|c}
		$A$ & $B$ & $C$ & $D$ & $E$ & $G$ & $F$ \\
		\hline
		$w$ & $w$ & $w$ & $w$ & $f$ & $f$ & $w$ \\
		$w$ & $f$ & $f$ & $w$ & $f$ & $w$ & $f$ \\
		$f$ & $w$ & $f$ & $w$ & $f$ & $w$ & $f$ \\
		$f$ & $f$ & $f$ & $f$ & $w$ & $w$ & $f$ \\
	\end{tabular}
\end{frame}
